\documentclass[a4paper,10pt]{article}
\input{/home/frr/UFSC/Pagina/Dropbox/Modelos/Modelo_prova_latex/estilo_prova.tex}

\begin{document}


\professor{Fábio Rodrigues de la Rocha}
\turma{06655}
\codigodisciplina{ARA7546}
\disciplina{Circuitos Digitais}
\data{02/04/2014}
\hlimite{20:20}
\listaexercicios{3}

\begin{center}
\large{\fbox{\mbox{Mapas de Karnaugh}}}
\end{center}

\questao{Simplifique as seguintes equações usando mapas K:}
\begin{enumerate}
 \item $f(A,B,C)=\sum{} m(0,2,3)$
 \item $f(A,B,C)=\sum{} m(1,2,4,6,7)$
 \item $f(A,B,C)=\sum{} m(0,1,2,3)$
 \item $f(A,B,C)=\sum{} m(0,2,4,6)$
 \item $f(A,B,C)=\sum{} m(0,3,5,6)$
 
 \item $f(A,B,C,D)=\overline{A}\,\overline{B}\,C+A\,D+B\overline{D}+C\,\overline{D}+A\,\overline{C}+\overline{A}\,\overline{B}$
 \item $f(A,B,C,D)=(A+B+\overline{C})(\overline{B}+\overline{D})(\overline{A}+C)(B+C)$
 \item $f(A,B,C,D)=\prod{} M(0,5,7,13,14,15)$
 \item $f(A,B,C,D)=\prod{} M(1,4,6,8,11,13,14)$
 \item $f(A,B,C,D)=\prod{} M(1,2,4,5,7,8,10,11,13,14)$
 \item $f(A,B,C,D)=\prod{} M(0,5,7,8,9,10,11,13)$
 \item $f(A,B,C,D)=\sum{} m(0,1,4,5,9,11,14,15)+d(10,13)$
 \item $f(A,B,C,D)=\sum{} m(0,13,14,15)+d(1,2,3,9,10,11)$
 \item $f(A,B,C,D)=\sum{} m(0,6,9,10,13)+d(1,3,8)$
 \item $f(A,B,C,D)=\sum{} m(1,4,7,10,13)+d(5,14,15)$
 
 
 
 
 
 \item $f(A,B,C,D,E)=\sum{} m(0,4,8,12,16,20,24,28)$
 \item $f(A,B,C,D,E)=\sum{} m(0,2,5,8,13,15,18,21,24,29,31)$
 \item $f(A,B,C,D,E)=\sum{} m(3,4,6,9,11,13,15,18,25,26,27,29,31)$
 \item $f(A,B,C,D,E)=\sum{} m(1,5,8,10,12,13,14,15,17,21,24,26,31)$
 \item $f(A,B,C,D,E)=A+B\,C+\overline{C}\,D\,\overline{E}$
 \item $f(A,B,C,D,E)=(A+B)(B+C)(C+\overline{D})(D+\overline{E})$
 \item $f(A,B,C,D,E)=\sum{} m(1,4,6,10,20,22,24,26)+d(0,11,16,17)$
 
 \item $f(A,B,C,D,E,F)=\prod{} M(2,3,6,7,10,14,18,19,22,23,27,37,42,43,45,46)$
 \item $f(A,B,C,D,E,F)=\prod{} M(6,9,13,18,19,25,27,29,41,45,57,61)$
 \item $f(A,B,C,D,E,F)=\prod{} M(4,5,6,7,8,18,20,23,25,26,27,28,37,38,42,44)$
 
 
 

 
 
 
 
 
 
 
\end{enumerate}





\end{document}